cleanup: use typeclass mechanism systematically for invariants

src/lib/state/DY.Lib.State.Tagged.fst
@@ -71,9 +71,9 @@ let split_local_bytes_state_predicate_params {|crypto_invariants|} : split_funct
 }
 
 [@@ "opaque_to_smt"]
-val has_local_bytes_state_predicate: protocol_invariants -> (string & local_bytes_state_predicate) -> prop
-let has_local_bytes_state_predicate invs (tag, spred) =
-  has_local_fun split_local_bytes_state_predicate_params (state_pred) (tag, spred)
+val has_local_bytes_state_predicate: {|protocol_invariants|} -> (string & local_bytes_state_predicate) -> prop
+let has_local_bytes_state_predicate #invs (tag, spred) =
+  has_local_fun split_local_bytes_state_predicate_params state_pred.pred (tag, spred)
 
 (*** Global tagged state predicate builder ***)
 
@@ -83,11 +83,11 @@ let mk_global_local_bytes_state_predicate #cinvs tagged_local_preds =
 
 #push-options "--ifuel 2" // to deconstruct nested tuples
 val mk_global_local_bytes_state_predicate_later:
-  cinvs:crypto_invariants -> tagged_local_preds:list (string & local_bytes_state_predicate) ->
+  {|crypto_invariants|} -> tagged_local_preds:list (string & local_bytes_state_predicate) ->
   tr1:trace -> tr2:trace -> prin:principal -> sess_id:state_id -> full_content:bytes -> Lemma
   (requires mk_global_local_bytes_state_predicate tagged_local_preds tr1 prin sess_id full_content /\ tr1 <$ tr2)
   (ensures mk_global_local_bytes_state_predicate tagged_local_preds tr2 prin sess_id full_content)
-let mk_global_local_bytes_state_predicate_later cinvs tagged_local_preds tr1 tr2 prin sess_id full_content =
+let mk_global_local_bytes_state_predicate_later #cinvs tagged_local_preds tr1 tr2 prin sess_id full_content =
   mk_global_fun_eq split_local_bytes_state_predicate_params tagged_local_preds (tr1, prin, sess_id, full_content);
   mk_global_fun_eq split_local_bytes_state_predicate_params tagged_local_preds (tr2, prin, sess_id, full_content);
   introduce forall lpred content. split_local_bytes_state_predicate_params.apply_local_fun lpred (tr1, prin, sess_id, content) ==> split_local_bytes_state_predicate_params.apply_local_fun lpred (tr2, prin, sess_id, content) with (
@@ -96,12 +96,12 @@ let mk_global_local_bytes_state_predicate_later cinvs tagged_local_preds tr1 tr2
 #pop-options
 
 val mk_global_local_bytes_state_predicate_knowable:
-  cinvs:crypto_invariants -> tagged_local_preds:list (string & local_bytes_state_predicate) ->
+  {|crypto_invariants|} -> tagged_local_preds:list (string & local_bytes_state_predicate) ->
   tr:trace -> prin:principal -> sess_id:state_id -> full_content:bytes ->
   Lemma
   (requires mk_global_local_bytes_state_predicate tagged_local_preds tr prin sess_id full_content)
   (ensures is_knowable_by (principal_state_label prin sess_id) tr full_content)
-let mk_global_local_bytes_state_predicate_knowable cinvs tagged_local_preds tr prin sess_id full_content =
+let mk_global_local_bytes_state_predicate_knowable #cinvs tagged_local_preds tr prin sess_id full_content =
   mk_global_fun_eq split_local_bytes_state_predicate_params tagged_local_preds (tr, prin, sess_id, full_content);
   match split_local_bytes_state_predicate_params.decode_tagged_data (tr, prin, sess_id, full_content) with
   | Some (tag, (_, _, _, content)) -> (
@@ -115,24 +115,24 @@ let mk_global_local_bytes_state_predicate_knowable cinvs tagged_local_preds tr p
   )
   | None -> ()
 
-val mk_state_pred: cinvs:crypto_invariants -> list (string & local_bytes_state_predicate) -> state_predicate cinvs
-let mk_state_pred cinvs tagged_local_preds =
+val mk_state_pred: {|crypto_invariants|} -> list (string & local_bytes_state_predicate) -> state_predicate
+let mk_state_pred #cinvs tagged_local_preds =
   {
     pred = mk_global_local_bytes_state_predicate tagged_local_preds;
-    pred_later = mk_global_local_bytes_state_predicate_later cinvs tagged_local_preds;
-    pred_knowable = mk_global_local_bytes_state_predicate_knowable cinvs tagged_local_preds;
+    pred_later = mk_global_local_bytes_state_predicate_later tagged_local_preds;
+    pred_knowable = mk_global_local_bytes_state_predicate_knowable tagged_local_preds;
   }
 
-val mk_state_pred_correct: invs:protocol_invariants -> tagged_local_preds:list (string & local_bytes_state_predicate) -> Lemma
+val mk_state_pred_correct: {|protocol_invariants|} -> tagged_local_preds:list (string & local_bytes_state_predicate) -> Lemma
   (requires
-    invs.trace_invs.state_pred == mk_state_pred invs.crypto_invs tagged_local_preds /\
+    state_pred == mk_state_pred tagged_local_preds /\
     List.Tot.no_repeats_p (List.Tot.map fst tagged_local_preds)
   )
-  (ensures for_allP (has_local_bytes_state_predicate invs) tagged_local_preds)
-let mk_state_pred_correct invs tagged_local_preds =
+  (ensures for_allP has_local_bytes_state_predicate tagged_local_preds)
+let mk_state_pred_correct #invs tagged_local_preds =
   reveal_opaque (`%has_local_bytes_state_predicate) (has_local_bytes_state_predicate);
   no_repeats_p_implies_for_all_pairsP_unequal (List.Tot.map fst tagged_local_preds);
-  for_allP_eq (has_local_bytes_state_predicate invs) tagged_local_preds;
+  for_allP_eq has_local_bytes_state_predicate tagged_local_preds;
   FStar.Classical.forall_intro_2 (FStar.Classical.move_requires_2 (mk_global_fun_correct split_local_bytes_state_predicate_params tagged_local_preds))
 
 (*** Predicates on trace ***)
@@ -164,14 +164,14 @@ let get_tagged_state the_tag prin sess_id =
       else return None
 
 val set_tagged_state_invariant:
-  invs:protocol_invariants ->
+  {|protocol_invariants|} ->
   tag:string -> spred:local_bytes_state_predicate ->
   prin:principal -> sess_id:state_id -> content:bytes -> tr:trace ->
   Lemma
   (requires
     spred.pred tr prin sess_id content /\
     trace_invariant tr /\
-    has_local_bytes_state_predicate invs (tag, spred)
+    has_local_bytes_state_predicate (tag, spred)
   )
   (ensures (
     let ((), tr_out) = set_tagged_state tag prin sess_id content tr in
@@ -180,23 +180,23 @@ val set_tagged_state_invariant:
   ))
   [SMTPat (set_tagged_state tag prin sess_id content tr);
    SMTPat (trace_invariant tr);
-   SMTPat (has_local_bytes_state_predicate invs (tag, spred))]
-let set_tagged_state_invariant invs tag spred prin sess_id content tr =
+   SMTPat (has_local_bytes_state_predicate (tag, spred))]
+let set_tagged_state_invariant #invs tag spred prin sess_id content tr =
   reveal_opaque (`%has_local_bytes_state_predicate) (has_local_bytes_state_predicate);
   reveal_opaque (`%set_tagged_state) (set_tagged_state);
   reveal_opaque (`%tagged_state_was_set) (tagged_state_was_set);
   let full_content = {tag; content;} in
   parse_serialize_inv_lemma #bytes tagged_state full_content;
-  local_eq_global_lemma split_local_bytes_state_predicate_params state_pred tag spred (tr, prin, sess_id, serialize _ full_content) tag (tr, prin, sess_id, content)
+  local_eq_global_lemma split_local_bytes_state_predicate_params state_pred.pred tag spred (tr, prin, sess_id, serialize _ full_content) tag (tr, prin, sess_id, content)
 
 val get_tagged_state_invariant:
-  invs:protocol_invariants ->
+  {|protocol_invariants|} ->
   tag:string -> spred:local_bytes_state_predicate ->
   prin:principal -> sess_id:state_id -> tr:trace ->
   Lemma
   (requires
     trace_invariant tr /\
-    has_local_bytes_state_predicate invs (tag, spred)
+    has_local_bytes_state_predicate (tag, spred)
   )
   (ensures (
     let (opt_content, tr_out) = get_tagged_state tag prin sess_id tr in
@@ -210,8 +210,8 @@ val get_tagged_state_invariant:
   ))
   [SMTPat (get_tagged_state tag prin sess_id tr);
    SMTPat (trace_invariant tr);
-   SMTPat (has_local_bytes_state_predicate invs (tag, spred))]
-let get_tagged_state_invariant invs tag spred prin sess_id tr =
+   SMTPat (has_local_bytes_state_predicate (tag, spred))]
+let get_tagged_state_invariant #invs tag spred prin sess_id tr =
   reveal_opaque (`%has_local_bytes_state_predicate) (has_local_bytes_state_predicate);
   reveal_opaque (`%get_tagged_state) (get_tagged_state);
   let (opt_content, tr_out) = get_tagged_state tag prin sess_id tr in
@@ -219,29 +219,29 @@ let get_tagged_state_invariant invs tag spred prin sess_id tr =
   | None -> ()
   | Some content ->
     let (Some full_content_bytes, tr) = get_state prin sess_id tr in
-    local_eq_global_lemma split_local_bytes_state_predicate_params state_pred tag spred (tr, prin, sess_id, full_content_bytes) tag (tr, prin, sess_id, content)
+    local_eq_global_lemma split_local_bytes_state_predicate_params state_pred.pred tag spred (tr, prin, sess_id, full_content_bytes) tag (tr, prin, sess_id, content)
 
 (*** Theorem ***)
 
 val tagged_state_was_set_implies_pred:
-  invs:protocol_invariants -> tr:trace ->
+  {|protocol_invariants|} -> tr:trace ->
   tag:string -> spred:local_bytes_state_predicate ->
   prin:principal -> sess_id:state_id -> content:bytes ->
   Lemma
   (requires
     tagged_state_was_set tr tag prin sess_id content /\
     trace_invariant tr /\
-    has_local_bytes_state_predicate invs (tag, spred)
+    has_local_bytes_state_predicate (tag, spred)
   )
   (ensures spred.pred tr prin sess_id content)
   [SMTPat (tagged_state_was_set tr tag prin sess_id content);
    SMTPat (trace_invariant tr);
-   SMTPat (has_local_bytes_state_predicate invs (tag, spred));
+   SMTPat (has_local_bytes_state_predicate (tag, spred));
   ]
-let tagged_state_was_set_implies_pred invs tr tag spred prin sess_id content =
+let tagged_state_was_set_implies_pred #invs tr tag spred prin sess_id content =
   reveal_opaque (`%has_local_bytes_state_predicate) (has_local_bytes_state_predicate);
   reveal_opaque (`%tagged_state_was_set) (tagged_state_was_set);
   let full_content = {tag; content;} in
   parse_serialize_inv_lemma #bytes tagged_state full_content;
   let full_content_bytes: bytes = serialize tagged_state full_content in
-  local_eq_global_lemma split_local_bytes_state_predicate_params state_pred tag spred (tr, prin, sess_id, full_content_bytes) tag (tr, prin, sess_id, content)
+  local_eq_global_lemma split_local_bytes_state_predicate_params state_pred.pred tag spred (tr, prin, sess_id, full_content_bytes) tag (tr, prin, sess_id, content)
